Various refactorings and cleanups
* Remove BlockTrace and bake everything into ChainTrace
* Simplify ChainTrace. Its signature is now
ChainTrace : Environment -> list Action -> Prop.

These changes will make it easier to reason over traces when proving
properties about contracts. For one, we can now talk about prefixes of
the entire chain without the weird distinction between block traces and
chain traces.

src/Blockchain.v
@@ -593,38 +593,7 @@ Proof.
 Qed.
 End Step.
 
-(* A block trace is essentially just the reflexive transitive closure of the steps.
-It captures execution within a single block. *)
-Inductive BlockTrace :
-  Environment -> list Action ->
-  Environment -> list Action -> Prop :=
-  | btrace_refl : forall {acts} {env : Environment},
-      BlockTrace env acts env acts
-  | btrace_step : forall {pre post} act tx mid new_acts suf final,
-      ChainStep pre act tx mid new_acts ->
-      BlockTrace mid (new_acts ++ suf) post final ->
-      BlockTrace pre (act :: suf) post final
-  | btrace_permute : forall pre post acts acts' final_acts,
-      Permutation acts acts' ->
-      BlockTrace pre acts post final_acts ->
-      BlockTrace pre acts' post final_acts.
-
-Section BlockTraceTheories.
-Context {pre : Environment} {acts : list Action}
-        {post : Environment} {post_acts : list Action}
-        (trace : BlockTrace pre acts post post_acts).
-
-Lemma block_header_post_steps : block_header post = block_header pre.
-Proof.
-  induction trace; auto.
-  match goal with
-  | [H: ChainStep _ _ _ _ _ |- _] => rewrite <- (block_header_post_step H)
-  end.
-  auto.
-Qed.
-End BlockTraceTheories.
-
-Definition add_new_block
+Definition add_new_block_header
           (header : BlockHeader)
           (baker : Address)
           (env : Environment) : Environment :=
@@ -640,6 +609,8 @@ let chain :=
          else blocks_baked chain a; |} in
 env <|env_chain := chain|>.
 
+(* Todo: this should just be a computation. But I still do not *)
+(* know exactly what the best way of working with reflect is *)
 Definition IsValidNextBlock (new old : BlockHeader) : Prop :=
   block_height new = S (block_height old) /\
   slot_number new > slot_number old /\
@@ -658,42 +629,44 @@ Definition initial_env :=
           contract_state a := None; |};
      env_contracts a := None; |}.
 
-Inductive ChainTrace : Environment -> Environment -> Prop :=
-| ctrace_initial :
-    forall (env : Environment),
-      EnvironmentEquiv env initial_env ->
-      ChainTrace env env
+(* The chain captures that an environment can be reached with some current actions. *)
+Inductive ChainTrace : Environment -> list Action -> Prop :=
+  | ctrace_initial :
+      forall (env : Environment),
+        EnvironmentEquiv env initial_env ->
+        ChainTrace env []
+  (* Add a new block to the trace *)
   | ctrace_block :
-      forall (prev_start prev_end : Environment)
+      forall (prev : Environment)
              (header : BlockHeader)
              (baker : Address)
              (acts : list Action)
-             (block_start new_end : Environment),
-        ChainTrace prev_start prev_end ->
-        IsValidNextBlock header (block_header prev_end) ->
+             (new : Environment),
+        ChainTrace prev [] ->
+        IsValidNextBlock header (block_header prev) ->
         Forall (fun act => address_is_contract (act_from act) = false) acts ->
-        BlockTrace block_start acts new_end [] ->
         EnvironmentEquiv
-          block_start
-          (add_new_block header baker prev_end) ->
-        ChainTrace prev_start new_end.
-
-Section ChainTraceTheories.
-Context {pre post : Environment} (trace : ChainTrace pre post).
-
-Lemma block_height_post_trace :
-  block_height (block_header pre) <= block_height (block_header post).
-Proof.
-  induction trace; auto.
-  match goal with
-  | [H: BlockTrace _ _ _ _, H': EnvironmentEquiv _ _ |- _]
-    => rewrite (block_header_post_steps H), H'
-  end.
-  unfold IsValidNextBlock in *.
-  simpl.
-  intuition.
-Qed.
-End ChainTraceTheories.
+          new
+          (add_new_block_header header baker prev) ->
+        ChainTrace new acts
+  (* Execute an action *)
+  | ctrace_step :
+      forall (prev : Environment)
+             (act : Action)
+             (acts : list Action)
+             (tx : Tx)
+             (new : Environment)
+             (new_acts : list Action),
+        ChainTrace prev (act :: acts) ->
+        ChainStep prev act tx new new_acts ->
+        ChainTrace new (new_acts ++ acts)
+  (* Reorder action order *)
+  | ctrace_permute :
+      forall (env : Environment)
+             (acts acts' : list Action),
+        ChainTrace env acts ->
+        Permutation acts acts' ->
+        ChainTrace env acts'.
 End Semantics.
 
 Class ChainBuilderType :=
@@ -713,7 +686,7 @@ Class ChainBuilderType :=
       option builder_type;
 
     builder_trace (b : builder_type) :
-      ChainTrace (builder_env builder_initial) (builder_env b);
+      ChainTrace (builder_env b) [];
   }.
 
 Global Coercion builder_type : ChainBuilderType >-> Sortclass.
